src/tls/HKDF.fst
@@ -7,61 +7,10 @@ open Hashing.Spec
 
 private let max (a:int) (b:int) = if a < b then b else a
 
-(*-------------------------------------------------------------------*)
-(*
-From https://tools.ietf.org/html/rfc5869
-
-HKDF-Extract(salt, IKM) -> PRK
-   Options:
-      Hash     a hash function; HashLen denotes the length of the
-               hash function output in octets
-   Inputs:
-      salt     optional salt value (a non-secret random value);
-               if not provided, it is set to a string of HashLen zeros.
-      IKM      input keying material
-   Output:
-      PRK      a pseudorandom key (of HashLen octets)
-
-   PRK = HMAC-Hash(salt, IKM)
-*)
-
-val hkdf_extract: ha:hash_alg -> salt:hkey ha -> ikm:bytes -> ST (tag ha)
-  (requires (fun h0 -> True))
-  (ensures (fun h0 t h1 -> FStar.HyperStack.modifies Set.empty h0 h1))
-
 let hkdf_extract ha salt ikm = HashMAC.hmac ha salt ikm
 
-
-(*-------------------------------------------------------------------*)
-(*
-HKDF-Expand(PRK, info, L) -> OKM
-   Options:
-      Hash     a hash function; HashLen denotes the length of the
-               hash function output in octets
-   Inputs:
-      PRK      a pseudorandom key of at least HashLen octets
-               (usually, the output from the extract step)
-      info     optional context and application specific information
-               (can be a zero-length string)
-      L        length of output keying material in octets (<= 255*HashLen)
-   Output:
-      OKM      output keying material (of L octets)
-
-   N = ceil(L/HashLen)
-   T = T(1) | T(2) | T(3) | ... | T(N)
-
-   OKM = first L octets of T
-
-   where:
-   T(0) = empty string
-   T(1) = HMAC-Hash(PRK, T(0) | info | 0x01)
-   T(2) = HMAC-Hash(PRK, T(1) | info | 0x02)
-   ...
-*)
-
-// we take a stricter approach and require that the secret and the hash have the same size.
 private val hkdf_expand_int: ha:hash_alg
-  -> prk: hkey ha //was: bytes{tagLen ha <= length prk} 
+  -> prk: hkey ha //was: bytes{tagLen ha <= length prk}
   -> info:bytes
   -> len:nat{len <= op_Multiply 255 (tagLen ha)}
   -> count:nat{count < 256 }
@@ -81,53 +30,16 @@ let rec hkdf_expand_int ha prk info len count curr prev =
     prev @| next
   else empty_bytes
 
-val hkdf_expand: ha:hash_alg
-  -> prk: hkey ha
-  -> info: bytes
-  -> len: nat{len <= op_Multiply 255 (tagLen ha)}
-  -> ST (lbytes len)
-  (requires (fun h0 -> True))
-  (ensures (fun h0 t h1 -> FStar.HyperStack.modifies Set.empty h0 h1))
-
 let hkdf_expand ha prk info len =
   lemma_repr_bytes_values len;
   let raw = hkdf_expand_int ha prk info len 0 0 empty_bytes in
   fst(split raw len)  // possibly chopping off the end of the last hash
 
-
-(*-------------------------------------------------------------------*)
-(*
-HKDF-Expand-Label(Secret, Label, Messages, Length) =
-       HKDF-Expand(Secret, HkdfLabel, Length)
-
-  Where HkdfLabel is specified as:
-
-  struct HkdfLabel {
-    uint16 length;
-    opaque label<9..255>;
-    opaque hash_value<0..255>;
-  };
-
-  - HkdfLabel.length is Length
-  - HkdfLabel.label is "TLS 1.3, " + Label
-  - HkdfLabel.hash_value is HashValue.
-*)
-
-val tls13_prefix: lbytes 9
 let tls13_prefix =
   let s = abytes "TLS 1.3, " in
   assume(length s = 9);
   //if length s <> 9 then Platform.Error.unexpected "Cannot be proved statically because abytes is underspecified";
   s
-
-val hkdf_expand_label: ha: hash_alg
-  -> prk: hkey ha
-  -> label: string{length (abytes label) < 256 - 9}
-  -> hv: bytes{length hv < 256}
-  -> len: nat{len <= op_Multiply 255 (tagLen ha)}
-  -> ST (lbytes len)
-  (requires (fun h0 -> True))
-  (ensures (fun h0 t h1 -> FStar.HyperStack.modifies Set.empty h0 h1))
 
 let hkdf_expand_label ha prk label hv len =
   let label_bytes = tls13_prefix @| abytes label in
